feat(KSA): KMS Decrypt/Encrypt Strategy (#1020)
Co-authored-by: Jose Corella <joseeduardocorella@gmail.com>

AwsCryptographicMaterialProviders/runtimes/net/Generated/AwsCryptographyKeyStoreAdmin/KeyManagementStrategy.cs
@@ -8,6 +8,7 @@ namespace AWS.Cryptography.KeyStoreAdmin
   public class KeyManagementStrategy
   {
     private AWS.Cryptography.KeyStore.AwsKms _awsKmsReEncrypt;
+    private AWS.Cryptography.KeyStoreAdmin.AwsKmsDecryptEncrypt _awsKmsDecryptEncrypt;
     public AWS.Cryptography.KeyStore.AwsKms AwsKmsReEncrypt
     {
       get { return this._awsKmsReEncrypt; }
@@ -17,9 +18,19 @@ namespace AWS.Cryptography.KeyStoreAdmin
     {
       return this._awsKmsReEncrypt != null;
     }
+    public AWS.Cryptography.KeyStoreAdmin.AwsKmsDecryptEncrypt AwsKmsDecryptEncrypt
+    {
+      get { return this._awsKmsDecryptEncrypt; }
+      set { this._awsKmsDecryptEncrypt = value; }
+    }
+    public bool IsSetAwsKmsDecryptEncrypt()
+    {
+      return this._awsKmsDecryptEncrypt != null;
+    }
     public void Validate()
     {
-      var numberOfPropertiesSet = Convert.ToUInt16(IsSetAwsKmsReEncrypt());
+      var numberOfPropertiesSet = Convert.ToUInt16(IsSetAwsKmsReEncrypt()) +
+      Convert.ToUInt16(IsSetAwsKmsDecryptEncrypt());
       if (numberOfPropertiesSet == 0) throw new System.ArgumentException("No union value set");
 
       if (numberOfPropertiesSet > 1) throw new System.ArgumentException("Multiple union values set");
